src/coq/StepSemantics.v
@@ -36,7 +36,7 @@ Module StepSemantics(A:ADDR).
     | DV : Expr dvalue -> dvalue
     | DVALUE_CodePointer (p : pc)
     | DVALUE_Addr (a:A.addr)
-    | DVALUE_I32 (x:CompCert.I32)
+(*    | DVALUE_I32 (x:CompCert.I32) *)
     .
   
     Module ET : Vellvm.Effects.EffT
@@ -105,7 +105,7 @@ Module StepSemantics(A:ADDR).
     | DV (VALUE_Integer i1), DV (VALUE_Integer i2) =>
       mret (DV (VALUE_Integer
                               match iop with
-                              | Add _ _ => (i1 + i2)%Zb
+                              | Add _ _ => (i1 + i2)%Z
                               | Sub _ _ => (i1 - i2)%Z
                               | Mul _ _ => (i1 * i2)%Z
                               | Shl _ _ 
